
\subsection{1D Rad Abs with drift $v\neq 0$}

Solution on an interval $[a,b]$, initial condition $p(z,z',t'=0)=\delta (z-z')$.

\newcommand{\rn}{\rho_n}

\paragraph{Green's function}
\begin{align}
  & p(z,t|z',t'=0) = 2e^{-\frac{1}{4D_1t}\left[v^2t^2 - 2(z-z')vt \right]}
      \sum_{n=0}^{\infty} e^{-D_1\rn^2t} \frac{ F_n(z')F_n(z) }
      {h + \left[\rn^2 + h^2\right]L}, \\
  &\quad\quad F_n(z) = h\sin\left(\rn(z-a)\right) +  \rn\cos\left(\rn(z-a)\right)  , \\
  &\quad\quad h = \frac{v/2 + k_+}{D_1}, \quad\quad L=(b-a), \quad\quad \tan\left(\rn L\right)=-\frac{\rn}{h}.
\end{align}

\paragraph{Survival probability}
\begin{align}
  S_z(t)
  &= \int_a^b pdz = 2e^{-\frac{1}{4D_1t}\left[ v^2t^2 + 2z'vt \right]} \\
  &\quad\quad
    \times\sum_{n=0}^{\infty} e^{-D_1\rn^2t}
    \frac{F_n(z')}{\Big. h + \left[\rn^2 + h^2\right]L \Big.}
    \frac{
    \left[
	  e^{\frac{va}{2D_1}} h \frac{k_+}{D_1}
	- e^{\frac{vb}{2D_1}} \left(\rn^2 + h^2\right) \cos(\rn L)
    \right]
    }
    {\frac{h}{\rn}\left[ \rn^2 + \frac{v^2}{4 D_1^2} \right]}.
\end{align}

\paragraph{Propensity function}
\begin{align}
  q_{z=0}(t) &= k_+ p|_{z=a} = 2k_+ e^{-\frac{1}{4D_1t}\left[v^2t^2 - 2(a-z')vt \right]} 
  \sum_{n=0}^{\infty} e^{-D_1\rn^2t}
  \frac{ \rn F_n(z')} {h + \left[\rn^2 + h^2\right]L}, \\
  q_{z=L}(t) &= \left.- D_1 \pd{p}{z}\right|_{z=b} \\
  &=  -2D_1 e^{-\frac{1}{4D_1t}\left[v^2t^2 - 2(b-z')vt \right]} 
    \sum_{n=0}^{\infty} e^{-D_1\rn^2t}
    \frac{F_n(z') \left[\frac{1}{h}\rn^3 + h\rn\right]\cos\left(\rn L\right)
 }
  {h + \left[\rn^2 + h^2\right]L}.
\end{align}

\paragraph{Cumulative Green's function}
\begin{multline}
 P(Z,t|z',t'=0) = \int_a^Z pdz \\
 \shoveleft{
  = 2e^{-\frac{1}{4D_1t}\left[ v^2t^2 + 2z'vt \right]}
    \sum_{n=0}^{\infty} e^{-D_1\rn^2t} \left\lbrace \frac{F_n(z')}{\Big. h + \left[\rn^2 + h^2\right]L \Big.} \right.
 } \\
 \shoveright{
    \quad\quad\quad \left.\times
    \frac{
    \left[
	  e^{\frac{va}{2D_1}} h\frac{k_+}{D_1}
	- e^{\frac{vZ}{2D_1}}
	    \left\lbrace
	       h\frac{k_+}{D_1}\cos\left(\rn(Z-a)\right) - \left(h\rn + \frac{h^2}{\rn}\frac{v}{2D_1}\right)\sin\left(\rn(Z-a)\right)
	    \right\rbrace
    \right]
    }
    {\frac{h}{\rn}\left[ \rn^2 + \frac{v^2}{4 D_1^2} \right]}
    \right\rbrace .
 }
\end{multline}
